updates on homework 6 and added haskell exercise

homework07/Haskell/src/Typeclasses.hs
@@ -1,0 +1,488 @@
+{-# LANGUAGE InstanceSigs #-}
+
+module Typeclasses where
+
+import Prelude hiding (fail, elem)
+import qualified Data.Map as M
+import Control.Monad hiding (fail)
+
+import Debug.Trace
+{- 
+
+Typeclasses
+-----------
+
+If we let Haskell infer the type of the following function, it will not be
+the one we wrote for it in the previous section, but something more general.
+
+-}
+  
+add :: Num a => a -> a -> a
+add = (+)
+
+{- 
+The above type tells us that add works for any type, as long as this type
+implements the [Num] type class. 
+
+What is a type class?
+
+A type class is a set of operations (functions and constants), can must be
+implemented by any type that is an _instance_ of the type class. Type class
+defines a common interface 
+
+Then when writing polymorphic functions, one can put constraints on
+polymorphic types that they should implement a particular type class. This is
+called a type class constraint. Then the function can access all the
+operations of the type class.
+
+Haskell implements overloading, which is the ability to define an operation
+for more than one types, using type classes. 
+
+The Num typeclass defines operations like +, -, * for numeric types. Every
+type that implements the typeclass, i.e., provides an instance of the type
+class, should define this operations.
+
+Another useful class is Eq, that defines equality and inequality.
+Its definition in Haskell library is the following:
+
+
+class Eq a where
+    (==)        :: a -> a -> Bool
+    (/=)        :: a -> a -> Bool
+
+    x /= y      = not (x == y) -- default implementation
+
+
+The definition of inequality has a default has a default implementation that 
+will be used when if the instance does not redefine the operation.
+
+Most build-in datatypes in Haskell provide instances for Eq But when we are
+defining our own types, we may want them to provide instances of such
+classes.
+
+-}
+
+data Tree a = Leaf | Node a (Tree a) (Tree a)
+
+-- The type class instance for Tree a, has a type class constraint that the
+-- type a must implement Eq
+
+instance Eq a => Eq (Tree a) where
+    (==) :: Eq a => Tree a -> Tree a -> Bool
+    Leaf          == Leaf             = True
+    Node a1 t1 t2 == Node a1' t1' t2' = a1 == a1' && t1 == t1' && t2 == t2'
+    _             ==                  _ = False 
+
+tree1 :: Tree Int
+tree1 = Node 42 (Node 17 Leaf Leaf) Leaf
+
+tree2 :: Tree Int 
+tree2 = Node 17 (Node 11 Leaf Leaf) Leaf
+
+--- >>> tree1 == tree2
+-- False
+
+--- >>> tree1 == tree1
+-- True
+
+-- Haskell lets us use the keyword deriving to automatically derive some
+-- instances. In Haskell 98, the only derivable classes are Eq, Ord, Enum, Ix,
+-- Bounded, Read, and Show. Various language extensions extend this list.
+
+-- For example:
+
+data Tree' a = Leaf' | Node' a (Tree' a) (Tree' a)
+  deriving (Eq, Show)
+
+tree1' :: Tree' Int
+tree1' = Node' 42 (Node' 17 Leaf' Leaf') Leaf'
+
+tree2' :: Tree' Int 
+tree2' = Node' 17 (Node' 11 Leaf' Leaf') Leaf'
+
+--- >>> tree1' == tree2'
+-- False
+
+--- >>> tree1' == tree1'
+-- True
+
+-- The Show type class provides one function show :: a -> String that converts
+-- its input to a string. 
+
+-- >>> show tree1'
+-- "Node' 42 (Node' 17 Leaf' Leaf') Leaf'"
+
+-- These derived instances might not always be the desired ones.
+
+-- For example, consider the following simple AST that contains information
+-- about the position of the node in the source code. When we compare
+-- expressions, we would like to ignore this.
+
+-- The source code position
+type Posn = (Int,Int) -- a type synonym
+
+data Exp = Var Posn String 
+         | App Posn Exp Exp
+         | Abs Posn String Exp
+         | Num Posn Int
+         | Add Posn Exp Exp 
+   deriving Show
+
+instance Eq Exp where
+    (==) :: Exp -> Exp -> Bool
+    Var _ x     == Var _ x'      = x == x'
+    App _ e1 e2 == App _ e1' e2' = e1 == e1' && e2 == e2'
+    Abs _ x e   == Abs _ x' e'   = x == x' && e == e'
+    Num _ n     == Num _ n'      = n == n'
+    Add _ e1 e2 == Add _ e1' e2' = e1 == e1' && e2 == e2'
+    _ == _ = False
+
+-- >>> (Add (0,2) (Num (0,0) 3) (Num (0,4) 4)) == (Add (1,2) (Num (1,0) 3) (Num (1,4) 4))
+-- True
+
+-- Another common typeclass is the Ord typeclass that provides comparison
+-- functions.
+
+-- Using Ord we can write a generic quicksort function
+
+qsort :: Ord a => [a] -> [a] -- What is Ord?
+qsort [] = []
+qsort (p:xs) =
+  qsort [x | x <- xs, x < p] ++
+  [p] ++ qsort [x | x <- xs, x >= p]
+
+
+{- 
+
+To summarize we've see four very standard type classes in Haskell:
+
+- Ord  : provides total orderings on data types
+- Show : allows data types to be printed as strings
+- Eq   : provides (in)equality operations
+- Num  : provides functionality common to all kinds of numbers
+
+Next, we will move to another very common Haskell typeclass: Monads.
+-}
+
+{- 
+
+Monads
+------
+
+Monads can be seen as a generic interface to various types of computations.
+
+This interface can be used to simulate an imperative programming style in purely 
+functional languages by hiding a lot of . This makes it easier to write code 
+that manipulates state, throws errors, models nondeterminism, etc.
+
+Monads can also be used to encapsulate truly impure code and keep it 
+separate from the pure language fragment (like the IO monad). 
+
+The interface that must be implemented by a monad is the following. 
+
+class Monad (m :: Type -> Type) where    
+  -- encapsulate a pure computation in a monadic one
+  return :: a -> m a
+  -- sequence two monadic compuations
+  (>>=)  :: m a -> (a -> m b) -> m b
+
+Note, that the monad is not parametric on a type, but a type operator. As we
+will see, this can be a List, a Maybe, or a "side-effect" type like IO.
+
+In addition to the interface, monads should satisfy the _monad laws_:
+
+return a >>= k = k a
+m >>= return = m 
+m >>= (\x -> k x >>= h)  =  (m >>= k) >>= h
+
+Note: As of 2017, Haskell require every Monad to also be an Applicative
+instance, and every Applicative to also have a Functor instance. to be 
+
+-}
+
+-- The Maybe Monad
+
+{- The implementation of the Maybe monad, provided by the Haskell standard library 
+   is the following:
+
+instance Monad Maybe where
+   return      :: a -> Maybe a
+   return         =  Just
+
+   (>>=)       :: Maybe a -> (a -> Maybe b) -> Maybe b
+   Nothing  >>= _ =  Nothing
+   (Just x) >>= f =  f x
+
+-}
+
+-- There is also a "monadic action" specific to this monad
+fail :: Maybe a
+fail = Nothing
+
+-- We can use the Maybe monad to avoid boilerplate code when writing recursive
+-- functions that return optional types. 
+
+-- For example we can write an interpreter for lambda calculus, which is a
+-- partial function, without having to explicitly match the result to get it out 
+-- of the Maybe type. We can simply use monadic bind to do this.
+
+subst :: String -> Exp -> Exp -> Exp 
+subst x t' t@(Var _ y)    = if x == y then t' else t
+subst x t' t@(Abs p y t1) = if x == y then t else Abs p y (subst x t' t1)
+subst x t' (App p t1 t2)  = App p (subst x t' t1) (subst x t' t2)
+subst _ _ t@(Num _ _)     = t
+subst x t' (Add p t1 t2)  = Add p (subst x t' t1) (subst x t' t2)
+
+psn :: Posn
+psn = (0,0)
+
+exp1 :: Exp
+exp1 = subst "x" (Abs psn "z" (Var psn "z")) (App psn (Var psn "x") (Add psn (Num psn 1) (Num psn 2)))
+
+-- >>> exp1
+-- App (0,0) (Abs (0,0) "z" (Var (0,0) "z")) (Add (0,0) (Num (0,0) 1) (Num (0,0) 2))
+
+eval :: Exp -> Maybe Exp
+eval (Var _ _) = fail
+eval (Abs p x t) = return (Abs p x t)  
+eval (App _ t1 t2) = 
+  eval t1 >>= (\v -> 
+    case v of
+      Abs _ x t -> 
+        eval t2 >>= (\v2 ->
+        eval (subst x v2 t))
+      _ -> fail)
+eval (Num p n) = return (Num p n)
+eval (Add p t1 t2) = 
+  eval t1 >>= (\v1 ->
+  eval t2 >>= (\v2 ->
+  case (v1, v2) of 
+    (Num _ n1, Num _ n2) -> return $ Num p (n1 + n2)
+    _ -> Nothing))
+
+-- >>> eval exp1
+-- Just (Num (0,0) 3)
+
+{-- 
+
+Do notation
+-----------
+
+This already feels all lot like sequencing imperative code. Haskell provides a
+"do notation" to makes this sequencing feel even more natural. 
+
+A monadic bind operation 
+
+m >>= \x -> m' 
+
+in do notation becomes 
+
+x <- m
+m'
+
+This notation, which resembles an imperative program, must be written inside a
+do block. The following example demonstrates this.  
+-}
+
+
+-- eval with do notation
+
+eval' :: Exp -> Maybe Exp
+eval' (Var _ _) = fail
+eval' (Abs p x t) = return (Abs p x t)  
+eval' (App _ t1 t2) = do
+  v <- eval' t1;
+  case v of
+    Abs _ x t -> do
+      v2 <- eval' t2;
+      eval (subst x v2 t)
+    _ -> fail
+eval' (Num p n) = return (Num p n)
+eval' (Add p t1 t2) = do 
+  v1 <- eval' t1;
+  v2 <- eval' t2;
+  case (v1, v2) of 
+    (Num _ n1, Num _ n2) -> return $ Num p (n1 + n2)
+    _ -> fail
+
+
+
+{-
+
+Generic Monad Functions 
+------------------------
+
+There are several monadic combinators that let us manipulate and sequence monadic computation. 
+Some examples are: 
+
+-- Map each element of a structure to a monadic action, evaluate these actions from left to 
+-- right, and collect the results. 
+mapM :: (Traversable t, Monad m) => (a -> m b) -> t a -> m (t b)
+
+-- Evaluate each monadic action in the structure from left to right, and collect the results. 
+sequence :: (Traversable t, Monad m) => t (m a) -> m (t a)
+
+-- Lift a pure function to a monadic one 
+liftM :: Monad m => (a1 -> r) -> m a1 -> m r
+
+-- Lift a pure function with two arguments to a monadic one 
+liftM2 :: Monad m => (a1 -> a2 -> r) -> m a1 -> m a2 -> m r
+
+-}   
+
+{- 
+
+The Reader Monad 
+----------------
+
+The reader monad encapsulates a computation that reads from a context. 
+When writing a program inside a reader monad we don't have to explicitly pass
+the context to each call, the context is treated as a global, read-only state.
+
+-}
+
+newtype Reader env a = Reader { runReader :: env -> a }
+
+instance Functor (Reader env) where
+  fmap f r = Reader (f . runReader r)
+
+instance Applicative (Reader env) where
+  pure x                   = Reader (\_ -> x)
+  Reader fe <*> Reader ae  = Reader (\e -> fe e (ae e))
+
+instance Monad (Reader env) where
+  (>>=) :: Reader env a -> (a -> Reader env b) -> Reader env b
+  x >>= f  = Reader $ \e -> let x' = runReader x e in runReader (f x') e
+
+ask :: Reader env env
+ask = Reader (\e -> e)
+
+
+-- For example, we can write the substitution function in a reader monad, to
+-- avoid explicitly passing the variable and expression to be substituted.
+
+substR :: Exp -> Reader (String, Exp) Exp 
+substR t@(Var _ y) = do
+   (x, t') <- ask
+   if x == y then return t' else return t
+substR t@(Abs p y t1) = do 
+  (x, _) <- ask
+  if x == y then return t
+  else liftM (Abs p y) (substR t1)
+substR (App p t1 t2)  = liftM2 (App p) (substR t1) (substR t2)
+substR t@(Num _ _)    = return t
+substR (Add p t1 t2)  = liftM2 (Add p) (substR t1) (substR t2)
+
+
+subst' :: String -> Exp -> Exp -> Exp
+subst' x t' t = runReader (substR t) (x,t')
+
+-- >>> subst' "x" (Abs psn "z" (Var psn "z")) (App psn (Var psn "x") (Add psn (Num psn 1) (Num psn 2)))
+-- App (0,0) (Abs (0,0) "z" (Var (0,0) "z")) (Add (0,0) (Num (0,0) 1) (Num (0,0) 2))
+  
+{- 
+
+The State Monad 
+----------------
+
+The reader monad encapsulates a computation that reads from a context. 
+When writing a program inside a reader monad we don't have to explicitly pass
+the context to each call, the context is treated as a global, read-only state.
+
+-}
+
+
+newtype State state a = State { runState :: state -> (state, a) }
+
+instance Functor (State state) where
+  fmap f st = State (\s -> let (s', a) = runState st s in (s', f a))
+
+instance Applicative (State state) where
+  pure x                 = State (\s -> (s,x))
+  State fs <*> State as  = State (\s -> 
+      let (s', f) = fs s in
+      let (s'', a) = as s' in (s'', f a))
+
+instance Monad (State state) where
+  (>>=) :: State state a -> (a -> State state b) -> State state b
+  x >>= f = State $ \s -> let (s', x') = runState x s in runState (f x') s'
+
+get :: State state state
+get = State (\s -> (s,s))
+
+put :: state -> State state ()
+put s = State (\_ -> (s,()))
+
+
+-- Example: Fibonacci as a stateful function
+
+type FibState = State (Integer, Integer)
+
+fibS :: Integer -> State (Integer, Integer) ()
+fibS 0 = pure ()
+fibS n = do 
+  fibS (n-1)
+  (curr, prev) <- get
+  put (curr + prev, curr)
+  pure ()
+
+
+getFibN :: Integer -> Integer
+getFibN = fst . fst . flip runState (0,1) . fibS
+
+-- >>> getFibN 8
+-- 21
+
+-- An (arguably) clearer version of the above would be:
+getFibN' :: Integer -> Integer
+getFibN' n = fib 
+  where
+    ((fib, _), _) = runState (fibS n) (0,1)
+
+-- >>> getFibN' 9
+-- 34
+
+-- We can also write this as a "for loop"
+
+fibNFor :: Integer -> Integer
+fibNFor n = snd . flip runState (0,1) $ do
+  
+  forM_ [0..(n-1)] $ \_ -> do
+    (curr,prev) <- get
+    put (curr+prev,curr)
+  
+  (curr,_) <- get
+  return curr
+
+-- >>> fibNFor 9
+-- 34
+
+
+{- Monad Transformers -}
+
+-- WIP 
+
+{- For example, we can write an environment-based interpreter without passing the context around. -}
+
+-- evalEnv :: Exp -> State Env Exp
+-- evalEnv (Var _ _) = f
+--   env <- get ;; 
+--   case M.lookup 
+-- evalEnv (Abs p x t) = return (Abs p x t)  
+-- evalEnv (App _ t1 t2) = do
+--   env <- get ;; 
+--   v <- evalEnv t1;
+--   case v of
+--     Abs _ x t -> do
+--       v2 <- evalEnv t2;
+--       put $ M.insert x v2 env
+--       evalEnv t
+--     _ -> fail
+-- evalEnv (Num p n) = return (Num p n)
+-- evalEnv (Add p t1 t2) = do 
+--   v1 <- evalEnv t1;
+--   v2 <- evalEnv t2;
+--   case (v1, v2) of 
+--     (Num _ n1, Num _ n2) -> return $ Num p (n1 + n2)
+--     _ -> fail
+
